[WIP] Try some more...

lang/Lang.v
@@ -785,6 +785,17 @@ Inductive ModSem: Type :=
               handler: forall E, (OHState owned_heap) ~> stateT owned_heap (itree E);
               sem: CallExternalE ~> itree (CallExternalE +' Event +' (OHState owned_heap)) }.
 
+Fixpoint ohs_to_OHState (ohs: list Any): Type -> Type :=
+  match ohs with
+  | [] => void1
+  | hd :: tl => OHState (projT1 hd) +' ohs_to_OHState tl
+  end
+.
+Inductive ModSemUnified (ohs: list Any): Type :=
+  mk_ModSemUnified
+    { genvU: string -> bool ;
+      (* customE: Type -> Type ; *)
+      semU: CallExternalE ~> itree (CallExternalE +' Event +' (ohs_to_OHState ohs)) }.
 (* Definition internal_to_external (c: CallInternalE val): CallExternalE val := *)
 (*   let '(CallInternal func_name args) := c in CallExternal (func_name) (args) *)
 (* . *)
@@ -802,7 +813,8 @@ Definition external_to_internal: CallExternalE ~> CallInternalE :=
 Definition eval_program2 (p: program): ModSem
   := mk_ModSem 
        (fun func_name => List.in_dec Strings.String.string_dec func_name (List.map fst p))
-       tt (* YJ: I want to use void1, but "initial_owned_heap" prevents me from doing that.
+       tt
+       (* YJ: I want to use void1, but "initial_owned_heap" prevents me from doing that.
 TODO: see if it is possible: don't require "initial_owned_heap", instead require "(handler initial_owned_heap)".
            *)
        (fun _ _ e _ => match e with | GetOH => Ret (tt, tt) | SetOH _ => Ret (tt, tt) end)
@@ -810,40 +822,64 @@ TODO: see if it is possible: don't require "initial_owned_heap", instead require
           ITree.map snd (interp_imp (denote_program2 p (external_to_internal call)) []))
 .
 
-(* Section TMP. *)
-(* Variable modsems: list ModSem. *)
-(* Check (fun c => *)
-(*           let '(CallExternal func_name args) := c in *)
-(*           modsem <- unwrapU (List.find (fun modsem => modsem.(genv) func_name) modsems) ;; *)
-(*                  modsem.(sem) c): CallExternalE val -> itree (CallExternalE +' Event) val. *)
-(* (* Set Printing All. *) *)
-(* Check (fun T (c: CallExternalE T) => *)
-(*           let '(CallExternal func_name args) := c in *)
-(*           modsem <- @unwrapU (CallExternalE +' Event) _ _ *)
-(*                  (List.find (fun modsem => modsem.(genv) func_name) modsems) ;; *)
-(*                  modsem.(sem) c) *)
-(*   (* : CallExternalE ~> itree (CallExternalE +' Event) *) *)
-(*   : forall T, CallExternalE T -> itree (CallExternalE +' Event) T *)
-(* . *)
+Definition ohs (mss: list ModSem): list Any :=
+  List.map (fun ms => existT id _ ms.(owned_heap)) mss
+.
 
-(* Check (fun T (c: CallExternalE T) => *)
-(*           let '(CallExternal func_name args) := c in *)
-(*           match (List.find (fun modsem => modsem.(genv) func_name) modsems) with *)
-(*           | Some modsem => modsem.(sem) c *)
-(*           | None => triggerUB *)
-(*           end) *)
-(*   (* : CallExternalE ~> itree (CallExternalE +' Event) *) *)
-(*   : forall T, CallExternalE T -> itree (CallExternalE +' Event) T *)
-(* . *)
-(* End TMP. *)
+Require Import Program.
+Definition Any_dec (a0 a1: Any): {a0=a1} + {a0<>a1}.
+  destruct a0, a1.
+  simpl_depind.
+  destruct (excluded_middle_informative (x = x0)).
+  - clarify.
+    destruct (excluded_middle_informative (p = p0)).
+    + clarify. left. rewrite sigT_eta. ss.
+    + right. ii. simpl_depind. clarify.
+  - right. ii. simpl_depind.
+Defined.
 
-Definition eval_multimodule (modsems: list ModSem): itree Event val
+(* Global Instance ReSum_ohs ( *)
+Global Instance Embeddable_ohs (ohs: list Any) (oh: Any) (IN: in_dec Any_dec oh ohs) T:
+  Embeddable (OHState (projT1 oh) T) (ohs_to_OHState ohs T).
+ginduction ohs; ii; ss.
+des_ifs.
+- left. ss.
+- right. eapply IHohs; eauto.
+  des_sumbool. ss.
+Defined.
+
+Definition modsem_unificaton (mss: list ModSem): list (ModSemUnified (ohs mss)) :=
+  List.map (fun ms =>
+              if in_dec Any_dec (existT id _ (ms.(owned_heap))) (ohs mss)
+              then mk_ModSemUnified (ohs mss) ms.(genv) ms.(sem)
+              else mk_ModSemUnified (fun _ => false) (fun _ => ITree.spin)
+           ) mss
+.
+
+Definition eval_multimodule_aux (ohs: list Any) (mss: list (ModSemUnified ohs))
+  : itree (Event +' ohs_to_OHState ohs) val
+  :=
+  let sem: CallExternalE ~> itree (Event +' (ohs_to_OHState ohs)) :=
+      mrec (fun T (c: CallExternalE T) =>
+              let '(CallExternal func_name args) := c in
+              ms <- @unwrapU (CallExternalE +' Event +' (ohs_to_OHState ohs)) _ _
+                     (List.find (fun ms => ms.(genvU) func_name) mss) ;;
+                     ms.(semU) c)
+  in
+  sem _ (CallExternal "main" [])
+.
+
+Definition eval_multimodule (mss: list ModSem): itree Event val :=
+
+State.interp_state
+Definition eval_multimodule (mss: list ModSem): itree Event val
   :=
   let sem: CallExternalE ~> itree Event :=
       mrec (fun T (c: CallExternalE T) =>
               let '(CallExternal func_name args) := c in
-              modsem <- @unwrapU (CallExternalE +' Event) _ _
-                     (List.find (fun modsem => modsem.(genv) func_name) modsems) ;; modsem.(sem) c)
+              ms <- @unwrapU (CallExternalE +' Event) _ _
+                     (List.find (fun ms => ms.(genv) func_name) mss) ;;
+                     ms.(sem) c)
   in
   sem _ (CallExternal "main" [])
 .
